untangle

Untangle.v
@@ -7,364 +7,99 @@ Require Export SystemFR.ScalaDepSugar.
 Require Export SystemFR.ReducibilitySubtype.
 Require Export SystemFR.EquivalentContext.
 Require Export SystemFR.TOpenTClose.
-Require Export SystemFR.CloseLemmas.
-Require Export SystemFR.SubstitutionErase.
 Require Export SystemFR.TermListReducible.
-Require Export SystemFR.ReducibilityOpenEquivalent.
 Require Export SystemFR.FVLemmasClose.
 Require Export SystemFR.WFLemmasClose.
-Require Export SystemFR.InferMatch.
-Require Export SystemFR.ErasedQuant.
+Require Export SystemFR.Existss.
+Require Export SystemFR.NormalizationPi.
+Require Export SystemFR.NormalizationExists.
+Require Export SystemFR.TauProperty.
 
 Opaque reducible_values.
 
-Parameter T_key: tree.
-Parameter T_map: tree.
-Axiom key_fv: forall tag, pfv T_key tag = nil.
-Axiom map_fv: forall tag, pfv T_map tag = nil.
-Axiom wf_key: wf T_key 0.
-Axiom wf_map: wf T_map 0.
-Axiom is_erased_type_key: is_erased_type T_key.
-Axiom is_erased_type_map: is_erased_type T_map.
+Definition incomparable_keys keys : Prop :=
+  forall key1 key2, key1 ∈ keys -> key2 ∈ keys ->
+    key1 = key2 \/ (~ prefix key1 key2 /\ ~ prefix key2 key1).
 
-Definition T_trail: tree := T_prod T_key T_map.
+Definition apps fs ts := List.map (fun p => app (fst p) (snd p)) (combine fs ts).
 
-Hint Resolve wf_key: wf.
-Hint Resolve wf_map: wf.
+Inductive untangle: context -> tree -> tree -> Prop :=
+| UntangleFreshen:
+    forall Γ T T' template xs ys fs keys m,
+      is_erased_type template ->
+      wf template 0 ->
+      Forall (fun key => [ key : T_key ]v) keys ->
+      Forall (fun f => wf f 0) fs ->
+      Forall is_erased_term fs ->
+      functional (combine ys keys) ->
+      functional (combine keys ys) ->
+      incomparable_keys keys ->
+      ~ m ∈ fv template ->
+      length keys = length xs ->
+      length fs = length xs ->
+      length ys = length xs ->
+      (forall f, f ∈ fs -> m ∈ fv f -> False) ->
+      (forall y, y ∈ ys -> y ∈ support Γ -> False) ->
+      (forall y, y ∈ ys -> y ∈ fv template -> False) ->
+      (forall x, x ∈ xs -> x ∈ support Γ -> False) ->
+      (forall f, f ∈ fs -> subset (fv f) (support Γ)) ->
+      (forall f, f ∈ fs -> [ Γ ⊨ f : T_tau ]) ->
+      (forall x, x ∈ fv template -> x ∈ xs \/ x ∈ support Γ) ->
+      T  = substitute template
+        (List.combine xs (apps fs (List.map (fun key => append_key key (fvar m term_var)) keys))) ->
+      T' = substitute template
+        (List.combine xs (apps fs (List.map (fun y => fvar y term_var) ys))) ->
+      untangle Γ
+               (T_exists T_trail (close 0 T m))
+               (T_exists_vars ys T_trail T')
 
-Hint Resolve is_erased_type_key: erased.
-Hint Resolve is_erased_type_map: erased.
+| UntangleAbstract:
+    forall Γ T A,
+      is_erased_type A ->
+      is_erased_type T ->
+      wf T 1 ->
+      wf A 0 ->
+      subset (fv A) (support Γ) ->
+      subset (fv T) (support Γ) ->
+      [ Γ ⊨ tnil : A ] ->
+      untangle Γ (T_exists T_trail (shift_open 0 T (tlookup A (lvar 0 term_var)))) (T_exists A T)
 
-Lemma wf_trail: wf T_trail 0.
-Proof. steps; eauto with wf. Qed.
+| UntanglePi:
+    forall Γ S S' T T' x,
+      is_erased_type T ->
+      is_erased_type T' ->
+      wf T 1 ->
+      wf T' 1 ->
+      subset (fv T) (support Γ) ->
+      subset (fv T') (support Γ) ->
+      ~ x ∈ pfv S term_var ->
+      ~ x ∈ pfv S' term_var ->
+      ~ x ∈ pfv_context Γ term_var ->
+      untangle Γ S S' ->
+      untangle ((x, S') :: Γ) (open 0 T (fvar x term_var)) (open 0 T' (fvar x term_var)) ->
+      untangle Γ (T_arrow S T) (T_arrow S' T')
 
-Hint Resolve wf_trail: wf.
+| UntangleExists:
+    forall Γ S S' T T' x,
+      is_erased_type T ->
+      is_erased_type T' ->
+      wf T 1 ->
+      wf T' 1 ->
+      subset (fv T) (support Γ) ->
+      subset (fv T') (support Γ) ->
+      ~ x ∈ pfv S' term_var ->
+      ~ x ∈ pfv_context Γ term_var ->
+      untangle Γ S S' ->
+      untangle ((x, S') :: Γ) (open 0 T (fvar x term_var)) (open 0 T' (fvar x term_var)) ->
+      untangle Γ (T_exists S T) (T_exists S' T')
 
-Lemma is_erased_type_trail: is_erased_type T_trail.
-Proof. steps; eauto with erased. Qed.
+| UntangleSingleton:
+    forall Γ T T' t,
+      untangle Γ T T' ->
+      untangle Γ (T_singleton T t) (T_singleton T' t)
 
-Hint Resolve is_erased_type_trail: erased.
-
-Lemma substitute_map:
-  forall l tag, psubstitute T_map l tag = T_map.
-Proof.
-  intros; apply substitute_nothing5; eauto using map_fv.
-Qed.
-
-Lemma substitute_key:
-  forall l tag, psubstitute T_key l tag = T_key.
-Proof.
-  intros; apply substitute_nothing5; eauto using key_fv.
-Qed.
-
-Lemma substitute_trail:
-  forall l tag, psubstitute T_trail l tag = T_trail.
-Proof.
-  repeat step || rewrite substitute_map || rewrite substitute_key.
-Qed.
-
-Opaque T_trail.
-
-Definition app2 f a b := app (app f a) b.
-Definition app3 f a b c := app (app (app f a) b) c.
-
-(* tlookup: type -> T_trail -> T_top *)
-Parameter tlookup: tree -> tree -> tree.
-
-(* concat: T_key -> T_key -> T_key *)
-Parameter concat: tree -> tree -> tree.
-
-(* append_key: T_key -> T_trail -> T_trail *)
-Parameter append_key: tree -> tree -> tree.
-
-Axiom append_key_trail:
-  forall key trail,
-    [ key : T_key ]v ->
-    [ trail : T_trail ]v ->
-    [ append_key key trail : T_trail ]v.
-
-Axiom wf_append_key:
-  forall k t1 t2,
-    wf t1 k ->
-    wf t2 k ->
-    wf (append_key t1 t2) k.
-
-Axiom psubstitute_append_key:
-  forall t1 t2 l tag,
-    psubstitute (append_key t1 t2) l tag =
-    append_key (psubstitute t1 l tag) (psubstitute t2 l tag).
-
-Axiom pfv_append_key:
-  forall t1 t2 tag, pfv (append_key t1 t2) tag = pfv t1 tag ++ pfv t2 tag.
-
-Axiom is_erased_term_append_key:
-  forall t1 t2,
-    is_erased_term t1 ->
-    is_erased_term t2 ->
-    is_erased_term (append_key t1 t2).
-
-Hint Resolve wf_append_key: wf.
-Hint Resolve is_erased_term_append_key: erased.
-
-(* prefix: T_key -> T_key -> Prop *)
-Parameter prefix: tree -> tree -> Prop.
-
-Parameter empty_map: tree (* T_map *).
-Axiom empty_map_type: [ empty_map : T_map ].
-
-(* update: T_trail -> T_key -> T_trail -> T_trail *)
-(* `update old_trail key trail` returns `old_trail` where `trail` is now rooted at `key` *)
-Parameter update: tree -> tree -> tree -> tree.
-
-Axiom update_type:
-  forall old_trail key trail,
-    [ old_trail : T_trail ]v ->
-    [ key : T_key ]v ->
-    [ trail : T_trail ]v ->
-    [ update old_trail key trail : T_trail ]v.
-
-Axiom wf_update:
-  forall k t1 t2 t3,
-    wf t1 k ->
-    wf t2 k ->
-    wf t3 k ->
-    wf (update t1 t2 t3) k.
-
-Axiom psubstitute_update:
-  forall t1 t2 t3 l tag,
-    psubstitute (update t1 t2 t3) l tag =
-    update (psubstitute t1 l tag) (psubstitute t2 l tag) (psubstitute t3 l tag).
-
-Axiom pfv_update:
-  forall t1 t2 t3 tag,
-    pfv (update t1 t2 t3) tag = pfv t1 tag ++ pfv t2 tag ++ pfv t3 tag.
-
-Axiom is_erased_term_update:
-  forall t1 t2 t3,
-    is_erased_term t1 ->
-    is_erased_term t2 ->
-    is_erased_term t3 ->
-    is_erased_term (update t1 t2 t3).
-
-Hint Resolve wf_update: wf.
-Hint Resolve is_erased_term_update: erased.
-
-(* Terms that take a map and a key `k`, and only lookup the map on keys greater or
-   equal than `k` satisfy the following property, described by the type `T_tau` *)
-Parameter T_tau: tree.
-
-Lemma tau_property:
-  forall f trail key old_trail,
-    [ f : T_tau ] ->
-    [ old_trail : T_trail ]v ->
-    [ trail : T_trail ]v ->
-    [ key : T_key ]v ->
-    [ app f trail ≡ app f (append_key key (update old_trail key trail)) ].
-Proof.
-Admitted.
-
-Axiom tau_fv: forall tag, pfv T_tau tag = nil.
-Axiom wf_tau: wf T_tau 0.
-Axiom is_erased_type_tau: is_erased_type T_tau.
-
-Hint Resolve wf_tau: wf.
-Hint Resolve is_erased_type_tau: erased.
-
-Lemma substitute_tau:
-  forall l tag, psubstitute T_tau l tag = T_tau.
-Proof.
-  intros; apply substitute_nothing5; eauto using tau_fv.
-Qed.
-
-Ltac equivalent_refl :=
-  match goal with
-  | |- [ _ ≡ _ ] => apply equivalent_refl
-  end.
-
-(*
-Lemma tau2_example:
-  forall f1 f2 fresh_key1 fresh_key2 fresh_map1 fresh_map2 key1 key2,
-    [ f1 : T_tau ] ->
-    [ f2 : T_tau ] ->
-    [ key1 : T_key ] ->
-    [ key2 : T_key ] ->
-    [ fresh_key1 : T_key ] ->
-    [ fresh_key2 : T_key ] ->
-    [ fresh_map1 : T_map ] ->
-    [ fresh_map2 : T_map ] ->
-    [ prefix fresh_key1 fresh_key2 ≡ tfalse ] ->
-    [ prefix fresh_key2 fresh_key1 ≡ tfalse ] ->
-    exists map,
-      [ app2 f1 fresh_map1 fresh_key1 ≡ app2 f1 map key1 ] /\
-      [ app2 f2 fresh_map2 fresh_key2 ≡ app2 f2 map key2 ].
-Proof.
-  intros.
-  exists (update key1 fresh_key1 fresh_map1 (update key2 fresh_key2 fresh_map2 empty_map)); steps.
-  - pose proof (tau_property _ key1 fresh_key1 fresh_map1
-      (update key2 fresh_key2 fresh_map2 empty_map) H); auto.
-  - pose proof (tau_property _ key2 fresh_key2 fresh_map2
-      (update key1 fresh_key1 fresh_map1 empty_map) H0); auto.
-    eapply equivalent_trans; eauto;
-      repeat apply equivalent_app || apply update_spec || equivalent_refl;
-      eauto 2 using reducible_erased with step_tactic;
-      eauto 2 using reducible_wf with step_tactic;
-      eauto 2 using reducible_fv with step_tactic;
-      eauto using empty_map_type.
-Qed.
-*)
-
-Fixpoint T_existss n T1 T2 :=
-  match n with
-  | 0 => T2
-  | S n' => T_exists T1 (T_existss n' T1 T2)
-  end.
-
-Definition T_exists_vars xs T1 T2 :=
-  T_existss (List.length xs) T1 (closes 0 T2 (rev xs)).
-
-Lemma wfs_combine:
-  forall l1 l2 k T,
-    List.Forall (fun t => [ t : T ]) l2 ->
-    wfs (List.combine l1 l2) k.
-Proof.
-  induction l1; steps; eauto 3 with wf step_tactic.
-Qed.
-
-Lemma wf_var:
-  forall n k, wf (fvar n term_var) k.
-Proof. steps. Qed.
-
-Hint Resolve wf_var: wf.
-
-Lemma wfs_combine2:
-  forall xs f keys m,
-    wf f 0 ->
-    List.Forall (fun key => [ key : T_key ]) keys ->
-    wfs (List.combine xs (List.map (fun key : tree => app f (pp key (fvar m term_var))) keys)) 0.
-Proof.
-  induction xs; destruct keys; steps; eauto with wf.
-Qed.
-
-Lemma wfs_combine3:
-  forall xs f keys m,
-    wf f 0 ->
-    List.Forall (fun key => [ key : T_key ]) keys ->
-    wfs (List.combine xs (List.map (fun key : tree => app f (append_key key (fvar m term_var))) keys)) 0.
-Proof.
-  induction xs; destruct keys; steps; eauto with wf.
-Qed.
-
-Lemma wfs_combine4:
-  forall xs f ys,
-    wf f 0 ->
-    wfs (List.combine xs (List.map (fun y => app f (fvar y term_var)) ys)) 0.
-Proof.
-  induction xs; destruct ys; steps.
-Qed.
-
-Lemma wfs_combine5:
-  forall l1 l2 k,
-    List.Forall (fun t => wf t k) l2 ->
-    wfs (List.combine l1 l2) k.
-Proof.
-  induction l1; steps.
-Qed.
-
-Lemma lookup_combine_map:
-  forall eq_dec (xs: list nat) f l (t1 t2: tree) x,
-    lookup eq_dec (List.combine xs l) x = Some t1 ->
-    lookup eq_dec (List.combine xs (List.map f l)) x = Some t2 ->
-    t2 = f t1.
-Proof.
-  induction xs; repeat step; eauto.
-Qed.
-
-Lemma lookup_combine_some_none:
-  forall eq_dec (xs: list nat) (l1 l2: list tree) t x,
-    List.length l1 = List.length l2 ->
-    lookup eq_dec (List.combine xs l1) x = Some t ->
-    lookup eq_dec (List.combine xs l2) x = None ->
-    False.
-Proof.
-  induction xs; steps; eauto.
-Qed.
-
-Lemma psubstitute_texistss:
-  forall n T1 T2 l tag,
-    psubstitute (T_existss n T1 T2) l tag =
-    T_existss n (psubstitute T1 l tag) (psubstitute T2 l tag).
-Proof.
-  induction n; repeat step || rewrite_any.
-Qed.
-
-Lemma substitute_closes:
-  forall xs t l tag k,
-    (forall x, x ∈ support l -> x ∈ xs -> False) ->
-    pclosed_mapping l term_var ->
-    psubstitute (closes k t xs) l tag = closes k (psubstitute t l tag) xs.
-Proof.
-  induction xs;
-    repeat step || rewrite substitute_close by (steps; eauto);
-    try solve [ rewrite_any; steps; eauto ].
-Qed.
-
-Lemma psubstitute_texists_vars:
-  forall xs T1 T2 l tag,
-    (forall x, x ∈ support l -> x ∈ xs -> False) ->
-    pclosed_mapping l term_var ->
-    psubstitute (T_exists_vars xs T1 T2) l tag =
-    T_exists_vars xs (psubstitute T1 l tag) (psubstitute T2 l tag).
-Proof.
-  unfold T_exists_vars; intros; rewrite psubstitute_texistss; apply f_equal.
-  rewrite substitute_closes; repeat step || rewrite <- in_rev in *; eauto.
-Qed.
-
-Lemma subst_subst:
-  forall t l ts xs tag,
-    (forall x, x ∈ pfv t tag -> x ∈ support l -> False) ->
-    psubstitute (psubstitute t (List.combine xs ts) tag) l tag =
-    psubstitute t (List.combine xs (List.map (fun t' => psubstitute t' l tag) ts)) tag.
-Proof.
-  induction t; repeat step || t_equality;
-    eauto 4 using lookup_combine_some_none, List.map_length with exfalso;
-    try solve [ rewrite_any; steps; eapply_any; repeat step || list_utils; eauto ];
-    try solve [ eapply_anywhere lookup_combine_map; eauto ];
-    try solve [ t_lookup; eauto with exfalso ].
-Qed.
-
-Lemma support_combine:
-  forall A B (l1: list A) (l2: list B),
-    List.length l1 = List.length l2 ->
-    support (List.combine l1 l2) = l1.
-Proof.
-  induction l1; destruct l2; repeat step || apply f_equal.
-Qed.
-
-Lemma range_combine:
-  forall A B (l1: list A) (l2: list B),
-    List.length l1 = List.length l2 ->
-    range (List.combine l1 l2) = l2.
-Proof.
-  induction l1; destruct l2; repeat step || apply f_equal.
-Qed.
-
-Lemma subst_subst2:
-  forall t l ts xs tag,
-    length ts = length xs ->
-    (forall x, x ∈ xs -> x ∈ support l -> False) ->
-    pclosed_mapping l tag ->
-    psubstitute (psubstitute t (List.combine xs ts) tag) l tag =
-    psubstitute (psubstitute t l tag)
-                (List.combine xs (List.map (fun t' => psubstitute t' l tag) ts)) tag.
-Proof.
-  induction t; repeat step || t_equality;
-    eauto 4 using lookup_combine_some_none, List.map_length with exfalso;
-    try solve [ eapply_anywhere lookup_combine_map; eauto ];
-    try solve [ rewrite substitute_nothing5; eauto with fv ].
-
-  repeat step || t_lookup || rewrite support_combine in * by auto;
-    eauto with exfalso.
-Qed.
+| UntangleRefl: forall Γ T, untangle Γ T T
+.
 
 Lemma list_map_subst:
   forall l f t m v,
@@ -384,367 +119,6 @@ Lemma list_map_subst2:
 Proof.
   induction l; repeat step || t_substitutions || rewrite psubstitute_append_key || t_equality; eauto.
 Qed.
-
-Fixpoint opens k t reps :=
-  match reps with
-  | nil => t
-  | rep :: reps => opens (S k) (open k t rep) reps
-  end.
-
-Lemma is_erased_type_existss:
-  forall n T1 T2,
-    is_erased_type T1 ->
-    is_erased_type T2 ->
-    is_erased_type (T_existss n T1 T2).
-Proof.
-  induction n; repeat step || apply_any.
-Qed.
-
-Hint Resolve is_erased_type_existss: erased.
-
-Lemma open_existss:
-  forall n T1 T2 k rep,
-    wf T1 0 ->
-    open k (T_existss n T1 T2) rep =
-    T_existss n T1 (open (n + k) T2 rep).
-Proof.
-  induction n; steps; repeat step || t_equality || open_none || rewrite_any ||
-                             rewrite PeanoNat.Nat.add_succ_r.
-Qed.
-
-Lemma open_close3:
-  forall t k1 k2 x rep,
-    fv rep = nil ->
-    wf rep 0 ->
-    k1 <> k2 ->
-    open k1 (close k2 t x) rep =
-    close k2 (open k1 t rep) x.
-Proof.
-  induction t; repeat step || t_equality || rewrite_any || rewrite close_nothing2 by auto.
-Qed.
-
-Lemma open_closes:
-  forall xs x T v i,
-    fv v = nil ->
-    wf v 0 ->
-    wf T 0 ->
-    open (length xs + i) (closes i T (xs ++ x :: nil)) v =
-    closes i (psubstitute T ((x, v) :: nil) term_var) xs.
-Proof.
-  induction xs; repeat step || rewrite open_close; eauto with wf.
-  rewrite open_close3; steps; eauto with lia.
-  rewrite <- PeanoNat.Nat.add_succ_r.
-  rewrite_any; steps.
-Qed.
-
-Lemma open_closes_zero:
-  forall xs x T v,
-    fv v = nil ->
-    wf v 0 ->
-    wf T 0 ->
-    open (length xs) (closes 0 T (xs ++ x :: nil)) v =
-    closes 0 (psubstitute T ((x, v) :: nil) term_var) xs.
-Proof.
-  intros.
-  rewrite <- (PeanoNat.Nat.add_0_r (length xs)); eauto using open_closes.
-Qed.
-
-Lemma reducible_exists_vars:
-  forall xs ρ v vs T1 T2,
-    wf T1 0 ->
-    wf T2 0 ->
-    is_erased_type T1 ->
-    is_erased_type T2 ->
-    List.Forall (fun v => [ ρ | v : T1 ]v) vs ->
-    List.length xs = List.length vs ->
-    valid_interpretation ρ ->
-    (forall z v', z ∈ xs -> v' ∈ vs -> z ∈ fv v' -> False) ->
-    [ ρ | v : psubstitute T2 (List.combine xs vs) term_var ]v ->
-    [ ρ | v : T_exists_vars xs T1 T2 ]v.
-Proof.
-  induction xs; repeat step || t_substitutions.
-  unshelve epose proof
-    (IHxs ρ v l T1 (psubstitute T2 ((a,t) :: nil) term_var) _ _ _ _ _ _ _ _ _); steps; eauto;
-    try solve [
-      rewrite <- substitute_cons2; repeat step || rewrite support_combine in * by auto; eauto
-    ];
-    eauto 3 with erased step_tactic;
-    eauto 3 with wf step_tactic.
-
-  unfold T_exists_vars in *.
-  simp_red_goal; steps; eauto 4 with erased; eauto using reducible_values_closed.
-  exists t; repeat step || rewrite open_existss; eauto with erased fv wf.
-  rewrite <- rev_length at 2.
-  rewrite open_closes; steps; eauto with wf fv.
-Qed.
-
-Definition functional { A B } (m: map A B) :=
-  forall a b1 b2,
-    (a, b1) ∈ m ->
-    (a, b2) ∈ m ->
-    b1 = b2.
-
-Lemma functional_head:
-  forall A B a b1 b2 (m: map A B),
-    functional ((a, b1) :: m) ->
-    (a, b2) ∈ m ->
-    b1 = b2.
-Proof.
-  unfold functional; steps; eauto.
-Qed.
-
-Lemma functional_tail:
-  forall A B a b (m: map A B),
-    functional ((a, b) :: m) ->
-    functional m.
-Proof.
-  unfold functional; steps; eauto.
-Qed.
-
-Lemma functional_tail2:
-  forall A B a1 a2 b1 b2 (m: map A B),
-    functional ((a1, b1) :: (a2, b2) :: m) ->
-    functional ((a1, b1) :: m).
-Proof.
-  unfold functional; steps; eauto 6.
-Qed.
-
-Ltac destruct_refinement :=
-  match goal with
-  | H: { _: _ | _ } |- _ => destruct H
-  | H: { _: _ & _ } |- _ => destruct H
-  end.
-
-Definition get_or_else { A } (opt: option A) (a: A) :=
-  match opt with
-  | None => a
-  | Some x => x
-  end.
-
-Lemma lookup_some_in:
-  forall A (l: map nat A) x a,
-    lookup Nat.eq_dec l x = Some a ->
-    (x, a) ∈ l.
-Proof.
-  induction l; steps.
-Qed.
-
-Lemma in_map_in_support:
-  forall A B (l: map A B) p,
-    p ∈ l ->
-    (fst p) ∈ support l.
-Proof.
-  induction l; steps.
-Qed.
-
-Lemma functional_get_or_else:
-  forall T a b (m: map nat T),
-    functional m ->
-    functional (m ++ (a, get_or_else (lookup Nat.eq_dec m a) b) :: nil).
-Proof.
-  unfold functional, get_or_else;
-    repeat step || list_utils || t_lookup; eauto;
-    try solve [ apply_anywhere lookup_some_in; steps; eauto ];
-    try solve [ apply_anywhere in_map_in_support; steps; eauto ];
-    eauto using in_combine_l with exfalso.
-Qed.
-
-Lemma decide_empty:
-  forall T (l: list T), l = nil \/ ~ l = nil.
-Proof.
-  destruct l; steps; right; steps.
-Qed.
-
-Lemma lookup_support:
-  forall A (l: map nat A) x,
-   x ∈ support l ->
-   exists a, lookup Nat.eq_dec l x = Some a.
-Proof.
-  induction l; repeat step; eauto.
-Qed.
-
-Lemma lookup_support2:
-  forall A (l1 l2: map nat A) x,
-   (forall s t, lookup Nat.eq_dec l1 s = Some t <-> lookup Nat.eq_dec l2 s = Some t) ->
-   x ∈ support l1 ->
-   x ∈ support l2.
-Proof.
-  intros.
-  apply_anywhere lookup_support; repeat step.
-  pose proof (H x a); repeat step || t_lookup.
-Qed.
-
-Lemma equivalent_subst_snoc:
-  forall l1 l2 a b,
-    equivalent_subst l1 l2 ->
-    equivalent_subst
-      (l1 ++ (a, b) :: nil)
-      (l2 ++ (a, get_or_else (lookup Nat.eq_dec l2 a) b) :: nil).
-Proof.
-  unfold equivalent_subst, get_or_else;
-    repeat step || list_utils || t_lookup || t_lookupor ||
-           (rewrite obvious_lookup in * by auto);
-    try solve [ apply lookupWeaken; steps; apply_any; steps ];
-    try solve [ unshelve epose proof (H s _); eauto; steps ].
-
-  - rewrite obvious_lookup in *; repeat step || t_lookup.
-    + apply eq_sym in H8; unshelve epose proof (H s b); repeat step || t_lookup.
-    + clear_marked. rewrite H8 in H0.
-      unshelve epose proof (H s t); repeat step || t_lookup.
-  - apply obvious_lookup; repeat step; eauto using lookup_support2.
-Qed.
-
-Lemma support_nil:
-  forall A B (l: map A B), support l = nil <-> l = nil.
-Proof.
-  destruct l; steps.
-Qed.
-
-Lemma forall_inst:
-  forall A (P: A -> Prop) l x,
-    x ∈ l ->
-    Forall P l ->
-    P x.
-Proof.
-  repeat step || rewrite Forall_forall in *.
-Qed.
-
-Ltac forall_inst :=
-  match goal with
-  | H1: ?x ∈ ?l, H2: Forall ?P ?l |- _ =>
-    poseNew (Mark (x, H2) "forall_inst");
-    pose proof (forall_inst _ _ _ _ H1 H2)
-  end.
-
-Lemma range_append:
-  forall A B (l1 l2: map A B),
-    range (l1 ++ l2) = range l1 ++ range l2.
-Proof.
-  induction l1; repeat step.
-Qed.
-
-Lemma recombine:
-  forall A B (m: map A B),
-    combine (support m) (range m) = m.
-Proof.
-  induction m; steps.
-Qed.
-
-Lemma length_support:
-  forall A B (l: map A B), length (support l) = length l.
-Proof.
-  induction l; steps.
-Qed.
-
-Lemma length_range:
-  forall A B (l: map A B), length (range l) = length l.
-Proof.
-  induction l; steps.
-Qed.
-
-Ltac list_utils2 :=
-  rewrite map_length in * || rewrite support_nil in * || rewrite in_map_iff in * ||
-  rewrite range_append in * || rewrite range_combine in * ||
-  rewrite List.map_map in * || rewrite support_combine in * ||
-  rewrite length_support in * || rewrite length_range in * ||
-  rewrite length_zero_iff_nil in * ||
-  rewrite recombine in * ||
-  forall_inst.
-
-Lemma functionalize_helper:
-  forall n (l: map nat tree),
-   length l < n ->
-   exists l',
-     functional l' /\
-      (forall y, y ∈ range l' -> y ∈ range l) /\
-     support l = support l' /\
-     equivalent_subst l l'.
-Proof.
-  induction n; steps; try lia.
-  pose proof (decide_empty _ l); steps.
-  - unfold functional, equivalent_subst; exists nil; steps.
-  - unshelve epose proof (@exists_last _ l _);
-      repeat step || destruct_refinement.
-    unshelve epose proof (IHn x _); repeat step || rewrite app_length in *; try lia.
-    exists (l' ++ (n0, get_or_else (lookup Nat.eq_dec l' n0) t) :: nil);
-      repeat step || apply equivalent_subst_snoc || list_utils || list_utils2;
-      eauto 2 using functional_get_or_else.
-    unfold get_or_else; steps; eauto using lookupRange.
-Qed.
-
-Lemma functionalize:
-  forall (l: map nat tree),
-    exists l',
-      functional l' /\
-      (forall y, y ∈ range l' -> y ∈ range l) /\
-      support l = support l' /\
-      equivalent_subst l l'.
-Proof.
-  eauto using functionalize_helper.
-Qed.
-
-Lemma functionalize_subst:
-  forall t l tag,
-  exists l',
-    functional l' /\
-    psubstitute t l tag = psubstitute t l' tag.
-Proof.
-  intros.
-  pose proof (functionalize l); steps;
-    eauto using subst_permutation.
-Qed.
-
-Lemma reducible_exists_vars2_helper:
-  forall xs ρ v T1 T2,
-    wf T1 0 ->
-    wf T2 0 ->
-    is_erased_type T1 ->
-    is_erased_type T2 ->
-    valid_interpretation ρ ->
-    [ ρ | v : T_exists_vars xs T1 T2 ]v ->
-    (exists vs,
-      List.Forall (fun v => [ ρ | v : T1 ]v) vs /\
-      length vs = length xs /\
-      [ ρ | v : psubstitute T2 (combine xs vs) term_var ]v).
-Proof.
-  unfold functional; induction xs; repeat step || t_substitutions || simp_red_top_level_hyp;
-    eauto 2 with step_tactic.
-
-  rewrite open_existss in *; eauto with wf.
-  rewrite <- rev_length in * at 2.
-  rewrite open_closes in *; eauto with wf fv.
-  rewrite rev_length in *.
-
-  unshelve epose proof (IHxs _ _ _ _ _ _ _ _ _ H9); steps;
-    eauto 2 with wf step_tactic;
-    eauto 2 with erased step_tactic.
-
-  exists (a0 :: vs); steps; eauto.
-  rewrite substitute_cons2; repeat step || (erewrite reducible_val_fv in * by eauto).
-Qed.
-
-Lemma reducible_exists_vars2:
-  forall xs ρ v T1 T2,
-    wf T1 0 ->
-    wf T2 0 ->
-    is_erased_type T1 ->
-    is_erased_type T2 ->
-    valid_interpretation ρ ->
-    [ ρ | v : T_exists_vars xs T1 T2 ]v ->
-    (exists vs,
-      List.Forall (fun v => [ ρ | v : T1 ]v) vs /\
-      functional (combine xs vs) /\
-      length vs = length xs /\
-      [ ρ | v : psubstitute T2 (combine xs vs) term_var ]v).
-Proof.
-  intros.
-  apply_anywhere reducible_exists_vars2_helper; steps.
-  pose proof (functionalize (combine xs vs)); repeat step || list_utils2.
-  exists (range l'); repeat step || list_utils || list_utils2 || rewrite Forall_forall in *.
-  erewrite subst_permutation in * |-; eauto.
-Qed.
-
-Definition apps fs ts := List.map (fun p => app (fst p) (snd p)) (combine fs ts).
 
 Lemma combine_equivalent_wfs1:
   forall ts1 ts2 xs,
@@ -814,18 +188,6 @@ Proof.
     repeat step || list_utils || list_utils2; eauto.
 Qed.
 
-Lemma pfv_in_subst2:
-  forall T (l : list (nat * tree)) tag x,
-    pclosed_mapping l tag ->
-    x ∈ pfv (psubstitute T l tag) tag ->
-    ~x ∈ support l.
-Proof.
-  intros.
-  epose proof (fv_subst2 _ _ _ x H0);
-    repeat step || list_utils;
-    eauto using closed_mapping_fv.
-Qed.
-
 Lemma reducibility_equivalent_substititions_helper:
   forall xs T ρ v ts1 ts2,
     [ ρ | v : psubstitute T (combine xs ts1) term_var ]v ->
@@ -872,42 +234,6 @@ Proof.
     apply_anywhere H12; steps.
   - apply combine_wfs5; auto.
 Qed.
-
-Lemma find_snd:
-  forall A B a (l1: list A) (l2: list B),
-    a ∈ l1 ->
-    length l1 = length l2 ->
-    exists b, (a, b) ∈ combine l1 l2.
-Proof.
-  induction l1; repeat step || instantiate_any; eauto.
-  pose proof (IHl1 _ H1 H); steps; eauto.
-Qed.
-
-Ltac find_snd :=
-  match goal with
-  | H1: context[combine ?l1 ?l2],
-    H2: ?x ∈ ?l1 |- _ =>
-    poseNew (Mark (l1, l2) "first_snd");
-    unshelve epose proof (find_snd _ _ _ l1 l2 H2 _)
-  end.
-
-Lemma find_fst:
-  forall A B b (l1: list A) (l2: list B),
-    b ∈ l2 ->
-    length l1 = length l2 ->
-    exists a, (a, b) ∈ combine l1 l2.
-Proof.
-  induction l1; repeat step || instantiate_any; eauto.
-  apply_anywhere eq_sym; list_utils2; steps.
-Qed.
-
-Ltac find_fst :=
-  match goal with
-  | H1: context[combine ?l1 ?l2],
-    H2: ?x ∈ ?l2 |- _ =>
-    poseNew (Mark (l1, l2) "first_fst");
-    unshelve epose proof (find_fst _ _ _ l1 l2 H2 _)
-  end.
 
 Lemma reducibility_equivalent_substititions:
   forall xs T ρ v ts1 ts2,
@@ -1184,10 +510,6 @@ Proof.
     try solve [ erewrite_anywhere lookup_combine2; eauto; steps ].
 Qed.
 
-(* empty_trail: T_trail *)
-Parameter empty_trail: tree.
-Axiom empty_trail_type: [ empty_trail : T_trail ]v.
-
 Lemma is_erased_term_global_trail':
   forall keys vs acc0,
     is_erased_term acc0 ->
@@ -1334,68 +656,8 @@ Proof.
   intros; rewrite fvs_global_trail in *; steps; eauto using typed_fv'.
 Qed.
 
-(* update: T_trail -> T_key -> T_trail -> T_trail *)
-(* `update old_trail key trail` returns `old_trail` with `trail` rooted at position `key` *)
-
-(*
-(* `update`'s are commutative when keys are not prefixes of one another *)
-Axiom update_spec:
-  forall key1 fresh_key1 fresh_map1 key2 fresh_key2 fresh_map2 map,    [ key1 : T_key ] ->
-    [ key2 : T_key ] ->
-    [ fresh_key1 : T_key ] ->
-    [ fresh_key2 : T_key ] ->
-    [ fresh_map1 : T_map ] ->
-    [ fresh_map2 : T_map ] ->
-    [ map : T_map ] ->
-    [ prefix fresh_key1 fresh_key2 ≡ tfalse ] ->
-    [ prefix fresh_key2 fresh_key1 ≡ tfalse ] ->
-    [ update key1 fresh_key1 fresh_map1 (update key2 fresh_key2 fresh_map2 map) ≡
-      update key2 fresh_key2 fresh_map2 (update key1 fresh_key1 fresh_map1 map) ].
-*)
-
-Axiom update_commutative:
-  forall key1 key2 old_trail trail1 trail2,
-    [ key1 : T_key ]v ->
-    [ key2 : T_key ]v ->
-    [ trail1 : T_trail ]v ->
-    [ trail2 : T_trail ]v ->
-    [ old_trail : T_trail ]v ->
-    ~ prefix key1 key2 ->
-    ~ prefix key2 key1 ->
-      update (update old_trail key2 trail2) key1 trail1 =
-      update (update old_trail key1 trail1) key2 trail2.
-
-(*
-Axiom update_spec3:
-  forall key fresh_key fresh_map map key',
-    [ prefix key key' ≡ tfalse ] ->
-    [ tlookup map key' ≡ tlookup (update key fresh_key fresh_map map) key' ].
-*)
-
-(*
-Definition global_trail keys vs :=
-  fold_left (fun acc p => update acc (fst p) (snd p)) (combine keys vs) empty_trail.
-*)
-
-(*
-  lookup (snd trail) δ = lookup (snd (update map key trail)) (concat key δ)
-*)
-
-(*
-Axiom update_type:
-  forall old_trail key trail,
-    [ old_trail : T_trail ]v ->
-    [ key : T_key ]v ->
-    [ trail : T_trail ]v ->
-    [ update old_trail key trail : T_trail ]v.
-*)
-
 Notation "'υ'" := (fun (acc : tree) (p : tree * tree) => update acc (fst p) (snd p))
   (at level 0).
-
-Definition incomparable_keys keys : Prop :=
-  forall key1 key2, key1 ∈ keys -> key2 ∈ keys ->
-    key1 = key2 \/ (~ prefix key1 key2 /\ ~ prefix key2 key1).
 
 Lemma fold_left_update_move:
   forall keys trails old_trail key0 trail0,
@@ -1508,29 +770,8 @@ Proof.
     repeat step || apply global_trail_good_trail.
 Qed.
 
-Lemma functional_trans:
-  forall A B C (l1: list A) (l2: list B) (l3: list C),
-    length l1 = length l2 ->
-    length l2 = length l3 ->
-    functional (combine l1 l2) ->
-    functional (combine l2 l3) ->
-    functional (combine l1 l3).
-Proof.
-  unfold functional; repeat step.
-  - pose proof (in_combine_l _ _ _ _ H3).
-    pose proof (in_combine_r _ _ _ _ H3).
-    pose proof (in_combine_r _ _ _ _ H4).
-    repeat find_fst || step.
-    repeat step || find_fst || find_snd.
-    
-    instantiate_any.
-
-    apply_anywhere in_combine_l; repeat step || find_snd.
-
-    find_snd.
-    apply_anywhere in_combine_l; repeat step || find_snd.
-    find_snd.
-  - 
+Opaque T_trail.
+Opaque T_tau.
 
 Lemma untangle_freshen:
   forall Γ fs template xs ys keys m,
@@ -1540,6 +781,7 @@ Lemma untangle_freshen:
     Forall (fun f => wf f 0) fs ->
     Forall is_erased_term fs ->
     functional (combine ys keys) ->
+    functional (combine keys ys) ->
     incomparable_keys keys ->
     ~ m ∈ fv template ->
     length keys = length xs ->
@@ -1581,7 +823,7 @@ Proof.
       eauto using var_in_support.
     apply reducible_exists_vars with (List.map (fun key => append_key key a) keys);
       repeat step || apply wf_subst || apply subst_erased_type || list_utils || list_utils2 ||
-             forall_inst || (erewrite reducible_val_fv in * by eauto) ||
+             Forall_inst || (erewrite reducible_val_fv in * by eauto) ||
              apply wfs_combine8 || apply erased_terms_combine2 || rewrite pfv_append_key in *;
       eauto 3 with wf step_tactic;
       eauto with erased;
@@ -1689,54 +931,14 @@ Proof.
       try solve [ eapply satisfies_erased_terms; eauto; steps ].
 
     + apply in_combine_equivalent' with fs keys vs l; steps.
-      unfold open_reducible in *; repeat step.
-      unshelve epose proof (H14 f _ nil l _ _ _);
-        repeat step || rewrite substitute_tau in *.
+      * unfold open_reducible in *; repeat step.
+        unshelve epose proof (H16 f _ nil l _ _ _);
+          repeat step || rewrite substitute_tau in *.
+      * apply functional_trans with _ ys; steps.
 
     + instantiate_any; steps.
       clear_marked; apply_anywhere pfv_in_subst2; steps; eauto with fv.
 Qed.
-
-Axiom open_lookup:
-  forall k A t rep,
-    open k (tlookup A t) rep = tlookup (open k A rep) (open k t rep).
-
-Axiom substitute_lookup:
-  forall A t l tag,
-    psubstitute (tlookup A t) l tag =
-    tlookup (psubstitute A l tag) (psubstitute t l tag).
-
-Axiom wf_lookup:
-  forall k A t,
-    wf A k ->
-    wf t k ->
-    wf (tlookup A t) k.
-
-Hint Resolve wf_lookup: wf.
-
-Axiom is_erased_term_lookup:
-  forall A t,
-    is_erased_type A ->
-    is_erased_term t ->
-    is_erased_term (tlookup A t).
-
-Hint Resolve is_erased_term_lookup.
-
-Axiom lookup_type:
-  forall A trail,
-    [ trail : T_trail ]v ->
-    [ tlookup A trail : A ].
-
-Axiom lookup_onto:
-  forall a A,
-    [ a : A ]v ->
-    exists trail,
-      [ trail : T_trail ]v /\
-      [ tlookup A trail ≡ a ].
-
-Axiom lookup_fv:
-  forall A trail tag,
-    pfv (tlookup A trail) tag = pfv A tag ++ pfv trail tag.
 
 Lemma untangle_abstract:
   forall Γ T A,
@@ -1746,6 +948,7 @@ Lemma untangle_abstract:
     wf A 0 ->
     subset (fv A) (support Γ) ->
     subset (fv T) (support Γ) ->
+    [ Γ ⊨ tnil : A ] ->
     [ Γ ⊨ T_exists T_trail (shift_open 0 T (tlookup A (lvar 0 term_var))) = T_exists A T ].
 Proof.
   unfold open_equivalent_types, equivalent_types; intros;
@@ -1753,7 +956,7 @@ Proof.
 
   - rewrite substitute_open2 in *; repeat step || list_utils; eauto with wf.
     rewrite open_shift_open4 in *; repeat step || rewrite open_lookup in * || open_none.
-    rewrite no_shift_open in H12;
+    rewrite no_shift_open in H13;
       repeat step || apply subst_erased_type;
       eauto with wf;
       try solve [ eapply satisfies_erased_terms; eauto; steps ].
@@ -1764,14 +967,17 @@ Proof.
       repeat step || rewrite lookup_fv || list_utils ||
              apply subst_erased_type || t_substitutions ||
              (rewrite (substitute_nothing5 a) in * by auto) ||
-             rewrite substitute_lookup in * ||
+             rewrite substitute_lookup in * || apply lookup_type ||
              apply is_erased_term_lookup;
       eauto with erased wf fv;
       try solve [ eapply satisfies_erased_terms; eauto; steps ];
-      eauto using lookup_type;
       try solve [ apply reducible_value_expr; steps ].
 
-  - unshelve epose proof (lookup_onto _ _ H10);
+    unfold open_reducible in *; repeat step.
+    unshelve epose proof (H5 nil l _ _ _); steps;
+      eauto using reducible_expr_value with values.
+
+  - unshelve epose proof (lookup_onto _ _ H11);
       repeat step || simp_red_goal || apply subst_erased_type;
       try solve [ eapply satisfies_erased_terms; eauto; steps ];
       eauto 3 with erased.
@@ -1794,47 +1000,15 @@ Proof.
     rewrite (substitute_nothing5 trail); eauto with fv; eauto using equivalent_sym.
 Qed.
 
-(* Using the tau property, we can untangle *)
-Inductive untangle: context -> tree -> tree -> Prop :=
-| UntangleFreshen:
-    forall Γ T T' template xs ys fs keys m,
-      is_erased_type template ->
-      wf template 0 ->
-      Forall (fun key => [ key : T_key ]v) keys ->
-      Forall (fun f => wf f 0) fs ->
-      Forall is_erased_term fs ->
-      functional (combine ys keys) ->
-      ~ m ∈ fv template ->
-      length keys = length xs ->
-      length fs = length xs ->
-      length ys = length xs ->
-      (forall f, f ∈ fs -> m ∈ fv f -> False) ->
-      (forall y, y ∈ ys -> y ∈ support Γ -> False) ->
-      (forall y, y ∈ ys -> y ∈ fv template -> False) ->
-      (forall x, x ∈ xs -> x ∈ support Γ -> False) ->
-      (forall f, f ∈ fs -> subset (fv f) (support Γ)) ->
-      (forall f, f ∈ fs -> [ Γ ⊨ f : T_tau ]) ->
-      (forall x, x ∈ fv template -> x ∈ xs \/ x ∈ support Γ) ->
-      T  = substitute template
-        (List.combine xs (apps fs (List.map (fun key => append_key key (fvar m term_var)) keys))) ->
-      T' = substitute template
-        (List.combine xs (apps fs (List.map (fun y => fvar y term_var) ys))) ->
-      untangle Γ
-               (T_exists T_trail (close 0 T m))
-               (T_exists_vars ys T_trail T')
-
-| UntangleAbstract:
-    forall Γ T A,
-      is_erased_type A ->
-      is_erased_type T ->
-      wf T 1 ->
-      wf A 0 ->
-      subset (fv A) (support Γ) ->
-      subset (fv T) (support Γ) ->
-      untangle Γ (T_exists T_trail (shift_open 0 T (tlookup A (lvar 0 term_var)))) (T_exists A T)
-
-| UntangleRefl: forall Γ T, untangle Γ T T
-.
+Lemma untangle_singleton:
+   forall Θ Γ T T' t,
+     [ Θ; Γ ⊨ T = T' ] ->
+     [ Θ; Γ ⊨ T_singleton T t = T_singleton T' t ].
+Proof.
+  unfold open_equivalent_types, equivalent_types;
+    repeat step || simp_red || t_instantiate_sat3;
+    eauto with eapply_any.
+Qed.
 
 Lemma untangle_open_equivalent_types:
   forall Γ T1 T2,
@@ -1844,5 +1018,8 @@ Proof.
   induction 1; steps;
     eauto using open_equivalent_types_refl;
     eauto using untangle_freshen;
+    eauto using open_npi;
+    eauto using open_nexists_2;
+    eauto using untangle_singleton;
     eauto using untangle_abstract.
 Qed.
