Functional.v
@@ -1,0 +1,107 @@
+Require Import PeanoNat.
+Require Import Psatz.
+Require Import Coq.Lists.List.
+
+Require Export SystemFR.AssocList.
+Require Export SystemFR.SubstitutionLemmas.
+
+Definition functional { A B } (m: map A B) :=
+  forall a b1 b2,
+    (a, b1) ∈ m ->
+    (a, b2) ∈ m ->
+    b1 = b2.
+
+Lemma functional_head:
+  forall A B a b1 b2 (m: map A B),
+    functional ((a, b1) :: m) ->
+    (a, b2) ∈ m ->
+    b1 = b2.
+Proof.
+  unfold functional; steps; eauto.
+Qed.
+
+Lemma functional_tail:
+  forall A B a b (m: map A B),
+    functional ((a, b) :: m) ->
+    functional m.
+Proof.
+  unfold functional; steps; eauto.
+Qed.
+
+Lemma functional_tail2:
+  forall A B a1 a2 b1 b2 (m: map A B),
+    functional ((a1, b1) :: (a2, b2) :: m) ->
+    functional ((a1, b1) :: m).
+Proof.
+  unfold functional; steps; eauto 6.
+Qed.
+
+Lemma functional_get_or_else:
+  forall T a b (m: map nat T),
+    functional m ->
+    functional (m ++ (a, get_or_else (lookup Nat.eq_dec m a) b) :: nil).
+Proof.
+  unfold functional, get_or_else;
+    repeat step || list_utils || t_lookup; eauto;
+    try solve [ apply_anywhere lookup_some_in; steps; eauto ];
+    try solve [ apply_anywhere in_map_in_support; steps; eauto ];
+    eauto using in_combine_l with exfalso.
+Qed.
+
+Lemma functionalize_helper:
+  forall n (l: map nat tree),
+   length l < n ->
+   exists l',
+     functional l' /\
+      (forall y, y ∈ range l' -> y ∈ range l) /\
+     support l = support l' /\
+     equivalent_subst l l'.
+Proof.
+  induction n; steps; try lia.
+  pose proof (decide_empty _ l); steps.
+  - unfold functional, equivalent_subst; exists nil; steps.
+  - unshelve epose proof (@exists_last _ l _);
+      repeat step || destruct_refinement.
+    unshelve epose proof (IHn x _); repeat step || rewrite app_length in *; try lia.
+    exists (l' ++ (n0, get_or_else (lookup Nat.eq_dec l' n0) t) :: nil);
+      repeat step || apply equivalent_subst_snoc || list_utils || list_utils2;
+      eauto 2 using functional_get_or_else.
+    unfold get_or_else; steps; eauto using lookupRange.
+Qed.
+
+Lemma functionalize:
+  forall (l: map nat tree),
+    exists l',
+      functional l' /\
+      (forall y, y ∈ range l' -> y ∈ range l) /\
+      support l = support l' /\
+      equivalent_subst l l'.
+Proof.
+  eauto using functionalize_helper.
+Qed.
+
+Lemma functionalize_subst:
+  forall t l tag,
+  exists l',
+    functional l' /\
+    psubstitute t l tag = psubstitute t l' tag.
+Proof.
+  intros.
+  pose proof (functionalize l); steps;
+    eauto using subst_permutation.
+Qed.
+
+Lemma functional_trans:
+  forall A B C (l1: list A) (l2: list B) (l3: list C),
+    length l1 = length l2 ->
+    length l2 = length l3 ->
+    functional (combine l1 l2) ->
+    functional (combine l2 l3) ->
+    functional (combine l1 l3).
+Proof.
+  unfold functional; repeat step.
+  unshelve epose proof (combine_middle_point _ _ _ l1 l2 l3 a b1 _ _ H3); steps.
+  unshelve epose proof (combine_middle_point _ _ _ l1 l2 l3 a b2 _ _ H4); steps.
+  pose proof (H1 _ _ _ H6 H8); steps.
+  pose proof (H2 _ _ _ H7 H9); steps.
+Qed.
