Options.v
@@ -1,0 +1,5 @@
+Definition get_or_else { A } (opt: option A) (a: A) :=
+  match opt with
+  | None => a
+  | Some x => x
+  end.
